add order to states

TotalViperState.thy
@@ -55,12 +55,193 @@ definition empty_full_total_state :: "'a store \<Rightarrow> 'a total_trace \<Ri
    \<rparr>"
 
 
-section \<open>Destructors \<close>
+subsection \<open>Order\<close>
 
-subsection \<open>total_state\<close>
+definition less_eq_mask :: "'a abstract_mask \<Rightarrow> 'a abstract_mask \<Rightarrow> bool"
+  where "less_eq_mask m1 m2 \<equiv> \<forall>l. lte (m1 l) (m2 l)"
+
+definition less_mask :: "'a abstract_mask \<Rightarrow> 'a abstract_mask \<Rightarrow> bool"
+  where "less_mask m1 m2 \<equiv> (\<forall>l. lte (m1 l) (m2 l)) \<and> (\<exists>l. lt (m1 l) (m2 l))"
+
+lemma less_mask_less_eq_mask: "less_mask m1 m2 = (less_eq_mask m1 m2 \<and> \<not> less_eq_mask m2 m1)"
+  unfolding less_mask_def less_eq_mask_def
+  apply(transfer)
+  using linorder_not_less by blast
+
+lemma less_eq_mask_refl: "less_eq_mask m m"
+  unfolding less_eq_mask_def  
+  by (transfer) simp
+
+lemma less_eq_mask_transitive: "less_eq_mask m1 m2 \<Longrightarrow> less_eq_mask m2 m3 \<Longrightarrow> less_eq_mask m1 m3"
+  unfolding less_eq_mask_def
+  apply transfer
+  using dual_order.trans by blast
+
+lemma less_eq_mask_antisymmetric: "less_eq_mask m1 m2 \<Longrightarrow> less_eq_mask m2 m1 \<Longrightarrow> m1 = m2"
+  unfolding less_eq_mask_def
+  apply transfer
+  using order_antisym_conv by blast
 
 
-subsection \<open>full total state\<close>
+instantiation total_state_ext :: (type,type) order
+begin
+
+definition less_eq_total_state_ext :: "('a,'b) total_state_ext \<Rightarrow> ('a,'b) total_state_ext \<Rightarrow> bool"
+  where "\<phi>1 \<le> \<phi>2 \<equiv> 
+         get_hh_total \<phi>1 = get_hh_total \<phi>2 \<and>
+         get_hp_total \<phi>1 = get_hp_total \<phi>2 \<and>
+         less_eq_mask (get_mh_total \<phi>1) (get_mh_total \<phi>2) \<and>
+         less_eq_mask (get_mp_total \<phi>1) (get_mp_total \<phi>2) \<and>
+         total_state.more \<phi>1 = total_state.more \<phi>2"
+
+definition less_total_state_ext :: "('a,'b) total_state_ext \<Rightarrow> ('a,'b) total_state_ext \<Rightarrow> bool"
+  where "\<phi>1 < \<phi>2 \<equiv> 
+         get_hh_total \<phi>1 = get_hh_total \<phi>2 \<and>
+         get_hp_total \<phi>1 = get_hp_total \<phi>2 \<and>
+         ( (less_eq_mask (get_mh_total \<phi>1) (get_mh_total \<phi>2) \<and> less_mask (get_mp_total \<phi>1) (get_mp_total \<phi>2)) \<or>
+           (less_mask (get_mh_total \<phi>1) (get_mh_total \<phi>2) \<and> less_eq_mask (get_mp_total \<phi>1) (get_mp_total \<phi>2))) \<and>
+         total_state.more \<phi>1 = total_state.more \<phi>2"
+instance
+proof
+  fix x y z :: "('a,'b) total_state_ext"
+
+  show "(x < y) = (x \<le> y \<and> \<not> y \<le> x)"
+  proof
+    assume "x < y"
+    show "x \<le> y \<and> \<not> y \<le> x"
+    proof (rule conjI)
+      show "x \<le> y"
+        using \<open>x < y\<close> less_mask_less_eq_mask
+        unfolding less_total_state_ext_def less_eq_total_state_ext_def
+        by meson
+    next
+      show "\<not> y \<le> x"
+      using \<open>x < y\<close> less_mask_less_eq_mask
+      unfolding less_total_state_ext_def less_eq_total_state_ext_def
+      by metis
+    qed
+  next
+    assume "x \<le> y \<and> \<not> y \<le> x"
+    thus "x < y"
+      using less_mask_less_eq_mask
+      unfolding less_total_state_ext_def less_eq_total_state_ext_def
+      by metis
+  qed
+
+  show "x \<le> x"
+    unfolding less_eq_total_state_ext_def
+    using less_eq_mask_refl
+    by meson
+
+  show "x \<le> y \<Longrightarrow> y \<le> z \<Longrightarrow> x \<le> z"
+    unfolding less_eq_total_state_ext_def
+    using less_eq_mask_transitive
+    by metis
+  
+  show "x \<le> y \<Longrightarrow> y \<le> x \<Longrightarrow> x = y"
+    unfolding less_eq_total_state_ext_def
+    apply (rule total_state.equality)
+    using less_eq_mask_antisymmetric
+    by blast+
+qed
+
+end
+
+instantiation full_total_state_ext :: (type,type) order
+begin
+
+definition less_eq_full_total_state_ext :: "('a,'b) full_total_state_ext \<Rightarrow> ('a,'b) full_total_state_ext \<Rightarrow> bool"
+  where "\<omega>1 \<le> \<omega>2 \<equiv> 
+         get_store_total \<omega>1 = get_store_total \<omega>2 \<and>
+         dom (get_trace_total \<omega>1) = dom (get_trace_total \<omega>2) \<and>
+         (\<forall>lbl \<phi>1 \<phi>2. get_trace_total \<omega>1 lbl = Some \<phi>1 \<longrightarrow> get_trace_total \<omega>2 lbl = Some \<phi>2 \<longrightarrow>
+                      \<phi>1 \<le> \<phi>2) \<and>
+         get_total_full \<omega>1 \<le> get_total_full \<omega>2 \<and>
+         full_total_state.more \<omega>1 = full_total_state.more \<omega>2"
+
+definition less_full_total_state_ext :: "('a,'b) full_total_state_ext \<Rightarrow> ('a,'b) full_total_state_ext \<Rightarrow> bool"
+  where "\<omega>1 < \<omega>2 \<equiv> 
+           \<omega>1 \<le> \<omega>2 \<and>
+           ( 
+             (\<exists>lbl \<phi>1 \<phi>2.  get_trace_total \<omega>1 lbl = Some \<phi>1 \<and> get_trace_total \<omega>2 lbl = Some \<phi>2 \<and>
+                           \<phi>1 < \<phi>2) \<or>
+             get_total_full \<omega>1 < get_total_full \<omega>2 
+           )"
+
+instance
+proof
+  fix x y z :: "('a,'b) full_total_state_ext"
+
+  show "(x < y) = (x \<le> y \<and> \<not> y \<le> x)"
+  proof
+    assume "x < y"
+    show "x \<le> y \<and> \<not> y \<le> x"
+    proof (rule conjI)
+      show "x \<le> y"
+        using \<open>x < y\<close> 
+        unfolding less_full_total_state_ext_def
+        by simp
+    next
+      from \<open>x < y\<close>
+      show "\<not> y \<le> x"
+        unfolding less_full_total_state_ext_def less_eq_full_total_state_ext_def
+        by fastforce
+    qed
+  next
+    assume "x \<le> y \<and> \<not> y \<le> x"
+    thus "x < y"
+    unfolding less_full_total_state_ext_def less_eq_full_total_state_ext_def    
+    by force
+  qed
+
+  show "x \<le> x"
+    unfolding less_eq_full_total_state_ext_def
+    by auto
+
+  show "x \<le> y \<Longrightarrow> y \<le> z \<Longrightarrow> x \<le> z"
+    unfolding less_eq_full_total_state_ext_def
+    by (metis (mono_tags, opaque_lifting) domD domI dual_order.trans)
+
+  have *: "dom (get_trace_total x) = dom (get_trace_total y) \<Longrightarrow>
+        (\<forall>lbl \<phi>1 \<phi>2. get_trace_total x lbl = Some \<phi>1 \<longrightarrow> get_trace_total y lbl = Some \<phi>2 \<longrightarrow> \<phi>1 \<le> \<phi>2) \<Longrightarrow>
+        (\<forall>lbl \<phi>1 \<phi>2. get_trace_total y lbl = Some \<phi>1 \<longrightarrow> get_trace_total x lbl = Some \<phi>2 \<longrightarrow> \<phi>1 \<le> \<phi>2) \<Longrightarrow>
+        get_trace_total x = get_trace_total y" (is "?A1 \<Longrightarrow> ?A2 \<Longrightarrow> ?A3 \<Longrightarrow> ?goal")
+  proof (rule HOL.ext)
+    fix arg
+    assume "?A1" and "?A2" and "?A3"
+
+    show "get_trace_total x arg = get_trace_total y arg"
+    proof (cases "get_trace_total x arg = None")
+      case True
+      then show ?thesis using \<open>?A1\<close>
+        by (metis domIff)
+    next
+      case False
+      from this obtain \<phi>1 \<phi>2 where
+        "get_trace_total x arg = Some \<phi>1" and
+        "get_trace_total y arg = Some \<phi>2"
+        using \<open>?A1\<close>
+        by (metis domD domIff)
+
+      then show ?thesis 
+        using \<open>?A2\<close> \<open>?A3\<close>
+        by fastforce
+    qed
+  qed
+
+  show "x \<le> y \<Longrightarrow> y \<le> x \<Longrightarrow> x = y"
+    unfolding less_eq_full_total_state_ext_def
+    apply (rule full_total_state.equality)
+       apply blast
+    using *
+      apply blast
+     apply fastforce
+    by blast
+qed
+end
+
+subsection \<open>Destructors \<close>
+
 fun get_hh_total_full :: "'a full_total_state \<Rightarrow> 'a total_heap"
   where "get_hh_total_full \<omega> = get_hh_total (get_total_full \<omega>)"
 
